src/LTS.v
@@ -23,9 +23,9 @@ Inductive St: Set :=
 | conf: AnnoTerm -> Plc -> Evidence -> St
 | rem: Plc -> Plc -> St -> St
 | ls: St -> AnnoTerm -> St
-| bsl: nat -> St -> AnnoTerm -> Plc -> Evidence -> St
+(*| bsl: nat -> St -> AnnoTerm -> Plc -> Evidence -> St
 | bsr: nat -> Evidence -> St -> St
-| bp: nat -> St -> St -> St.
+| bp: nat -> St -> St -> St*).
 
 Fixpoint pl (s:St) :=
   match s with
@@ -33,9 +33,9 @@ Fixpoint pl (s:St) :=
   | conf _ p _ => p
   | rem _ p _ => p
   | ls st _ => pl st
-  | bsl _ _ _ p _ => p
+  (*| bsl _ _ _ p _ => p
   | bsr _ _ st => pl st
-  | bp _ _ st => pl st
+  | bp _ _ st => pl st *)
   end.
 
 (** The evidence associated with a state. *)
@@ -46,9 +46,9 @@ Fixpoint seval st :=
   | conf t p e => aeval t p e
   | rem _ _ st => seval st
   | ls st t => aeval t (pl st) (seval st)
-  | bsl _ st t p e => ss (seval st) (aeval t p e)
+  (*| bsl _ st t p e => ss (seval st) (aeval t p e)
   | bsr _ e st => ss e (seval st)
-  | bp _ st0 st1 => pp (seval st0) (seval st1)
+  | bp _ st0 st1 => pp (seval st0) (seval st1) *)
 end.
 
 (** * Labeled Transition System
@@ -96,7 +96,7 @@ Inductive step: St -> option Ev -> St -> Prop :=
     forall t p e,
       step (ls (stop p e) t) None (conf t p e)
 (** Branching Sequential Composition *)
-
+(*
 | stbseq:
     forall r s x y p e,
       step (conf (abseq r s x y) p e)
@@ -142,7 +142,7 @@ Inductive step: St -> option Ev -> St -> Prop :=
     forall j p e p' e',
       step (bp j (stop p e) (stop p' e'))
            (Some (join (pred j) p'))
-           (stop p' (pp e e')).
+           (stop p' (pp e e')) *).
 Hint Constructors step : core.
 
 (** A step preserves place. *)
@@ -277,6 +277,7 @@ Proof.
   eapply star_tran; eauto.
 Qed.
 
+(*
 Lemma star_stbsl:
   forall st0 st1 j t p e,
     star st0 st1 ->
@@ -309,6 +310,7 @@ Proof.
     eapply star_tran; eauto.
   - eapply star_tran; eauto.
 Qed.
+*)
 
 Theorem correct_path_exists:
   forall t p e,
@@ -326,6 +328,7 @@ Proof.
     apply star_stls.
     apply IHt1.
     eapply star_tran; eauto.
+    (*
   - eapply star_tran; eauto.
     eapply star_transitive.
     apply star_stbsl.
@@ -340,7 +343,7 @@ Proof.
     apply star_stbp.
     apply IHt1.
     apply IHt2.
-    eapply star_tran; eauto.
+    eapply star_tran; eauto. *)
 Qed.
 
 (** * Progress *)
@@ -367,10 +370,11 @@ Proof.
       eapply ex_intro; eauto.
     + exists None.
       eapply ex_intro; eauto.
+      (*
     + exists (Some (split (fst r) n)).
       eapply ex_intro; eauto.
     + exists (Some (split (fst r) n)).
-      eapply ex_intro; eauto.
+      eapply ex_intro; eauto. *)
   - right.
     destruct IHst0.
     + destruct st0; simpl in H; try tauto.
@@ -388,6 +392,7 @@ Proof.
       exists e.
       destruct H as [st H].
       exists (ls st a). auto.
+      (*
   - right.
     destruct IHst0.
     + destruct st0; simpl in H; try tauto.
@@ -420,7 +425,7 @@ Proof.
     + destruct H as [e0 H].
       exists e0.
       destruct H as [st H].
-      exists (bp n st st0_2). auto.
+      exists (bp n st st0_2). auto. *)
 Qed.
 
 (** * Termination *)
@@ -478,8 +483,8 @@ Fixpoint tsize t: nat :=
   | aasp _ _ => 1
   | aatt _ _ x => 2 + tsize x
   | alseq _ x y => 2 + tsize x + tsize y
-  | abseq _ _ x y => 3 + tsize x + tsize y
-  | abpar _ _ x y => 2 + tsize x + tsize y
+  (*| abseq _ _ x y => 3 + tsize x + tsize y
+  | abpar _ _ x y => 2 + tsize x + tsize y *)
   end.
 
 (** Size of a state (number of steps to reduce). *)
@@ -490,9 +495,9 @@ Fixpoint ssize s: nat :=
   | conf t _ _ => tsize t
   | rem _ _ x => 1 + ssize x
   | ls x t => 1 + ssize x + tsize t
-  | bsl _ x t _ _ => 2 + ssize x + tsize t
+  (*| bsl _ x t _ _ => 2 + ssize x + tsize t
   | bsr _ _ x => 1 + ssize x
-  | bp _ x y => 1 + ssize x + ssize y
+  | bp _ x y => 1 + ssize x + ssize y *)
   end.
 
 (** Halt state has size 0. *)
