src/Main.v
@@ -36,7 +36,7 @@ Inductive traceS: St -> list Ev -> Prop :=
     traceS st tr1 ->
     trace t (pl st) tr2 ->
     traceS (ls st t) (tr1 ++ tr2)
-| tbsl: forall st tr1 t p e tr2 j,
+(*| tbsl: forall st tr1 t p e tr2 j,
     traceS st tr1 ->
     trace t p tr2 ->
     traceS (bsl j st t p e)
@@ -50,7 +50,7 @@ Inductive traceS: St -> list Ev -> Prop :=
     traceS st1 tr1 -> traceS st2 tr2 ->
     shuffle tr1 tr2 tr3 ->
     traceS (bp j st1 st2)
-           (tr3 ++ [(join (pred j) (pl st2))]).
+           (tr3 ++ [(join (pred j) (pl st2))]) *).
 Hint Constructors traceS : core.
 
 Fixpoint esizeS s:=
@@ -59,9 +59,9 @@ Fixpoint esizeS s:=
   | conf t _ _ => esize t
   | rem _ _ st => 1 + esizeS st
   | ls st t => esizeS st + esize t
-  | bsl _ st t _ _ => 1 + esizeS st + esize t
+  (*| bsl _ st t _ _ => 1 + esizeS st + esize t
   | bsr _ _ st => 1 + esizeS st
-  | bp _ st1 st2 => 1 + esizeS st1 + esizeS st2
+  | bp _ st1 st2 => 1 + esizeS st1 + esizeS st2 *)
   end.
 
 Lemma esize_tr:
@@ -73,12 +73,13 @@ Proof.
   apply IHt in H5. lia.
   apply IHt1 in H5.
   apply IHt2 in H6. lia.
+  (*
   apply IHt1 in H6.
   apply IHt2 in H7. lia.
   apply shuffle_length in H8.
   apply IHt1 in H6.
-  apply IHt2 in H7.
-  lia.
+  apply IHt2 in H7. 
+  lia. *)
 Qed.
 
 Lemma esizeS_tr:
@@ -92,6 +93,7 @@ Proof.
   - rewrite app_length; simpl.
     apply IHst in H2. apply esize_tr in H4.
     lia.
+    (*
   - repeat (rewrite app_length; simpl).
     apply IHst in H6.
     apply esize_tr in H7. lia.
@@ -101,7 +103,7 @@ Proof.
     apply IHst1 in H3.
     apply IHst2 in H5.
     apply shuffle_length in H6.
-    lia.
+    lia. *)
 Qed.
 
 Lemma step_silent_tr:
@@ -129,6 +131,7 @@ Proof.
     rewrite G; auto. *)
   - rewrite <- app_nil_l with (l:=tr).
     constructor; auto.
+    (*
   - pose proof H8 as G.
     eapply IHst in H8; eauto.
     (*apply step_seval in G.
@@ -156,7 +159,7 @@ Proof.
     (* rewrite <- G; auto. *)
     apply step_pl_eq in G1.
     rewrite <- G1; auto.
-    apply tbp with (tr1:=tr1)(tr2:=tr2); auto.
+    apply tbp with (tr1:=tr1)(tr2:=tr2); auto. *)
 Qed.
 
 Lemma step_evt_tr:
@@ -170,10 +173,11 @@ Proof.
     constructor.
   - constructor. apply tatt. simpl.
     inv H4; auto.
+    (*
   - constructor. apply tbseq; auto.
     inv H6; auto.
   - constructor. eapply tbpar; eauto.
-    inv H3; auto. inv H5; auto.
+    inv H3; auto. inv H5; auto. *)
   - pose proof H6 as G.
     apply step_seval in G.
     pose proof H6 as G1.
@@ -191,6 +195,7 @@ Proof.
     rewrite app_comm_cons.
     apply tls; auto.
     (*rewrite G. *) rewrite G1; auto.
+    (*
   - pose proof H8 as G.
     apply step_seval in G.
     eapply IHst in H8; eauto.
@@ -221,7 +226,7 @@ Proof.
       (*rewrite <- G; *) rewrite <- G1; auto.
     apply tbp with (tr1:=tr1)(tr2:=(ev::tr2)); auto.
   - rewrite <- app_nil_l; auto.
-    apply tbp with (tr1:=[])(tr2:=[]); auto.
+    apply tbp with (tr1:=[])(tr2:=[]); auto. *)
 Qed.
 
 Lemma nlstar_trace_helper:
